Added UTF8Transform and addressed PR feedback

examples/src/StreamingToyExample.cs
@@ -1,0 +1,90 @@
+using System;
+using System.IO;
+using System.Text;
+using Xunit;
+using System.Linq;
+
+using ibyteseq = Dafny.ISequence<byte>;
+using IO;
+using STL;
+using AWSEncryptionSDK;
+
+namespace StreamingToyExample {
+
+    class StreamingToyExample {
+
+        static public void RunEncryptInStreamExample() {
+            String fileInput = "tmp/streaming-encrypt-input.txt";
+            String fileExpected = "tmp/streaming-encrypt-expected.txt";
+
+            // Read input file and perform transformation using Dafny Enumerator
+            // Note that in this example, we load all of the final message into memory
+            string encryptedMessage;
+            using (FileStream fsSource = new FileStream(fileInput, FileMode.Open, FileAccess.Read))
+            {
+                using (EncryptInStream fileEncryptor = new EncryptInStream(fsSource))
+                {
+                    using (StreamReader reader = new StreamReader(fileEncryptor)) {
+                        encryptedMessage = reader.ReadToEnd();
+                    }
+                }
+            }
+            
+            // Read expected output from file
+            String expected; 
+            using (FileStream fsSource = new FileStream(fileExpected, FileMode.Open, FileAccess.Read))
+            {
+                // Read bytes as UTF-8
+                using (StreamReader reader = new StreamReader(fsSource))
+                {
+                    expected = reader.ReadToEnd();
+                }
+            }
+
+            Assert.Equal(expected, encryptedMessage);
+        }
+
+        static public void RunEncryptOutStreamExample() {
+            // Hardcode a source file for now
+            String fileInput = "tmp/streaming-encrypt-input.txt";
+            String fileExpected = "tmp/streaming-encrypt-expected.txt";
+
+            // Read input file and perform transformation using Dafny Enumerator
+            string encryptedMessage;
+            MemoryStream toTest = new MemoryStream();
+            using (FileStream fsSource = new FileStream(fileInput, FileMode.Open, FileAccess.Read))
+            {
+                using (EncryptOutStream fileEncryptor = new EncryptOutStream(toTest))
+                {
+                    // Encrypt the file and move output to the MemoryStream
+                    fsSource.CopyTo(fileEncryptor);
+                    // Read the MemoryStream as a string
+                    using (StreamReader reader = new StreamReader(toTest))
+                    {
+                        // Reset position on MemoryStream so we can read
+                        toTest.Position = 0;
+                        encryptedMessage = reader.ReadToEnd();
+                    }
+                }
+            }
+
+            // Read expected output from file
+            String expected; 
+            using (FileStream fsSource = new FileStream(fileExpected, FileMode.Open, FileAccess.Read))
+            {
+                // Read bytes as UTF-8
+                using (StreamReader reader = new StreamReader(fsSource))
+                {
+                    expected = reader.ReadToEnd();
+                }
+            }
+
+            Assert.Equal(expected, encryptedMessage);
+        }
+
+        static void Main(string[] args) {
+            RunEncryptInStreamExample();
+            RunEncryptOutStreamExample();
+        }
+    }
+}
