src/api/dotnet/EncryptStream.cs
@@ -1,36 +1,39 @@
 using System;
 using System.IO;
+using ToyUTF8Transform;
 using IO;
 using STL;
 using ibyteseq = Dafny.ISequence<byte>;
 
 namespace AWSEncryptionSDK
 {
-    // EncryptStream maps a readable C# Stream to a Dafny BytesEnumerator
+    // EncryptInStream maps a readable C# Stream to a Dafny BytesEnumerator
     // which wraps another readable C# Stream.
     // TODO implement IDisposable
-    public class EncryptStream : Stream {
+    public class EncryptInStream : Stream {
+        // TODO: Implement ReadByte()
 
-        readonly private EncryptEnumerator encryptor;
+        readonly private ToyEnumerator encryptor;
         readonly private Stream sourceStream;
         private MemoryStream outBuffer;
         // We ust maintain EOF state here if interface errors on read after EOF
         private bool atEOF;
 
-        public EncryptStream(Stream sourceStream) {
+        public EncryptInStream(Stream sourceStream) {
             if (!sourceStream.CanRead) {
-                // TODO find the right or define new Exception type
-                throw new NotSupportedException("Source stream supplied does not support reading");
+                throw new ArgumentException("Source stream supplied does not support reading");
             }
             this.sourceStream = sourceStream;
 
-            // This is some weirdness, but I'm not sure if we'll be able to avoid it
+            // Set up the ToyEnumerator to work with the source stream
+            // The way we do this is weird, using a C# constructor for the extern and the generated constructor
+            // for the ToyEnumerator, but I'm not sure if we'll be able to avoid it
             var externWrapper = new ExternBytesEnumerator(sourceStream);
-            var encryptor = new EncryptEnumerator();
+            var encryptor = new ToyEnumerator();
             encryptor.__ctor(externWrapper);
 
             this.encryptor = encryptor;
-            this.outBuffer = new MemoryStream();
+            this.outBuffer = new MemoryStream(); // TODO the way I use MemoryStream is hacky, update to use byte[] efficiently?
             this.atEOF = false;
         }
 
@@ -92,7 +95,7 @@ namespace AWSEncryptionSDK
             }
             
             // If outBuffer is empty, we should fill it
-            if (outBuffer.Length <= 0) {
+            if (outBuffer.Length - outBuffer.Position <= 0) {
                 Option<ibyteseq> opt = DafnyFFI.ExtractResult(encryptor.Next());
                 if (opt is Option_None<ibyteseq> none) {
                     atEOF = true;
@@ -107,6 +110,7 @@ namespace AWSEncryptionSDK
             // TODO what error states might we want
             // to handle when wrapping a C# Read?
             var readLen = outBuffer.Read(buffer, offset, count);
+            // TODO if readLen is 0 here something is v wrong
             return readLen;
         }
 
@@ -123,6 +127,144 @@ namespace AWSEncryptionSDK
         public override void Write(byte[] buffer, int offset, int count)
         {
             throw new NotSupportedException();
+        }
+
+        protected override void Dispose(bool disposing)
+        {
+            // Note: the sinkStream is NOT dispoed if this object is, and anyone using this Stream must appropriately close it
+            // TODO any disposing specific logic?
+            // TODO what should we do if this closes early? Fail because they don't have a valid ciphertext?
+            // TODO should we also deallocate other managed resources, like the outBuffer?
+            try {
+                // TODO even if not disposing?
+                if (!atEOF) {
+                    // TODO create the right exception for this
+                    throw new Exception("EncryptStream closed before encryption finished.");
+                }
+            }
+            finally {
+                base.Dispose(disposing);
+            }
+        }
+
+    }
+
+    // EncryptOutStream maps a readable C# Stream to a Dafny BytesEnumerator
+    // which wraps another readable C# Stream.
+    // TODO implement IDisposable, should call End() on Dispose?
+    public class EncryptOutStream : Stream {
+        // TODO: Implement WriteByte()
+
+        readonly private ToyAggregator encryptor;
+        readonly private Stream sinkStream;
+
+        public EncryptOutStream(Stream sinkStream) {
+            if (!sinkStream.CanWrite) {
+                // TODO find the right or define new Exception type
+                throw new NotSupportedException("Source stream supplied does not support writing");
+            }
+            this.sinkStream = sinkStream;
+
+            // This is some weirdness, but I'm not sure if we'll be able to avoid it
+            var externWrapper = new ExternBytesAggregator(sinkStream);
+            var encryptor = new ToyAggregator();
+            encryptor.__ctor(externWrapper);
+
+            this.encryptor = encryptor;
+        }
+
+        public override bool CanRead
+        {
+            get
+            {
+                return false;
+            }
+        }
+
+        public override bool CanSeek
+        {
+            get
+            {
+                return false;
+            }
+        }
+
+        public override bool CanWrite
+        {
+            get
+            {
+                return true;
+            }
+        }
+
+        public override void Flush()
+        {
+          // MUST flush the underlying stream. This means that we must flush the underlying encryptor.
+          // In our case, we need to indicate End, as having data buffered means that we require more
+          // data in order to be valid. Without that data we are in a bad state. End() will appropraitely
+          // return an error. Otherwise, this will signal end and flush the sink Stream.
+          // TODO: What would foo being false mean?
+          bool foo = DafnyFFI.ExtractResult(encryptor.End());
+          sinkStream.Flush();
+        }
+
+        public override long Length
+        {
+            get
+            {
+                throw new NotSupportedException();
+            }
+        }
+
+        public override long Position
+        {
+            get
+            {
+                throw new NotSupportedException();
+            }
+            set
+            {
+                throw new NotSupportedException();
+            }
+        }
+
+        public override int Read(byte[] buffer, int offset, int count)
+        {
+            throw new NotSupportedException();
+        }
+
+        public override long Seek(long offset, SeekOrigin origin)
+        {
+            throw new NotSupportedException();
+        }
+
+        public override void SetLength(long value)
+        {
+            throw new NotSupportedException();
+        }
+
+        public override void Write(byte[] buffer, int offset, int count)
+        {
+            // TODO what does false foo mean?
+            var foo = DafnyFFI.ExtractResult(encryptor.Accept(DafnyFFI.SequenceFromByteArray(buffer, offset, count)));
+        }
+        
+        // The sinkStream is NOT managed by this object, and anyone using this Stream must appropriately close it
+        protected override void Dispose(bool disposing)
+        {
+            try {
+                // Release managed resources in encryptor by calling End(). In the ToyExample case, if
+                // there is anything in the buffer, we should error, because the bytes inputted
+                // were not valid UTF8. In the decrypt case, we want this sort of thing to happen
+                // if the user tries to end the stream before getting to the message signature. Ideally we
+                // would zero out the plaintext returned if we could, but in this case those bytes are out of
+                // our hands :( and into the outStream
+                // TODO disposing vs. not disposing?
+                // TODO: What would foo being false mean?
+                bool foo = DafnyFFI.ExtractResult(encryptor.End());
+            } finally {
+                base.Dispose(disposing);
+            }
         }
     }
 }
