src/extern/dotnet/IO.cs
@@ -6,7 +6,7 @@ using ibyteseq = Dafny.ISequence<byte>;
 
 namespace IO {
     public partial class ExternBytesEnumerator {
-        private Stream inputStream; //readonly?
+        readonly private Stream inputStream;
 
         readonly int MAX_READ_LEN = 4096; // arbitrary, currently what the Java ESDK uses
 
@@ -16,17 +16,47 @@ namespace IO {
 
         public Result<Option<ibyteseq>> NextExtern() {
             byte[] readBuffer = new byte[MAX_READ_LEN];
-            int readLen = inputStream.Read(readBuffer, 0, readBuffer.Length);
+            int readLen;
+            try {
+                readLen = inputStream.Read(readBuffer, 0, readBuffer.Length);
+            } catch (IOException e) {
+                return Result<Option<ibyteseq>>.create_Failure(DafnyFFI.DafnyStringFromString(e.Message));
+            } catch (ObjectDisposedException e) {
+                return Result<Option<ibyteseq>>.create_Failure(DafnyFFI.DafnyStringFromString(e.Message));
+            }
+                
             if (readLen == 0) {
-                // EOF
                 return Result<Option<ibyteseq>>.create_Success(DafnyFFI.NullableToOption<ibyteseq>(null));
             }
 
-            // Copy and trim read bytes into new sequence
-            byte[] byteChunk = new byte[readLen];
-            Array.Copy(readBuffer, 0, byteChunk, 0, readLen);
-            // And then they get copied again :).
-            return Result<Option<ibyteseq>>.create_Success(DafnyFFI.NullableToOption(DafnyFFI.SequenceFromByteArray(byteChunk)));
+            return Result<Option<ibyteseq>>.create_Success(DafnyFFI.NullableToOption(DafnyFFI.SequenceFromByteArray(readBuffer, 0, readLen)));
         }
     }
+
+    public partial class ExternBytesAggregator {
+        readonly private Stream outputStream;
+
+        public ExternBytesAggregator(Stream outputStream) {
+            this.outputStream = outputStream;
+        }
+
+        public Result<bool> AcceptExtern(ibyteseq element) {
+            try {
+                outputStream.Write(element.Elements, 0, element.Elements.Length);
+                return Result<bool>.create_Success(true);
+            } catch (IOException e) {
+                return Result<bool>.create_Failure(DafnyFFI.DafnyStringFromString(e.Message));
+            } catch (ObjectDisposedException e) {
+                return Result<bool>.create_Failure(DafnyFFI.DafnyStringFromString(e.Message));
+            }
+        }
+
+        public Result<bool> EndExtern() {
+            // TODO Should this flush the sink stream, or should the caller be responsible for flushing it?
+            // normally I'd say "yes", however things like CryptoStreams require you to FlushFinalFrame instead
+            // of Flush. Given this implementation in the wild, I think it's reasonable to expect the user to do
+            // this, as well as dispose the sink stream.
+            return Result<bool>.create_Success(true);
+        }
+    } 
 }
