src/StandardLibrary/Collections.dfy
@@ -1,0 +1,188 @@
+include "StandardLibrary.dfy"
+include "UInt.dfy"
+include "../Util/UTF8.dfy"
+
+module {:extern "Collections"} Collections {
+  import opened StandardLibrary
+  import opened UInt = StandardLibrary.UInt
+
+  trait {:termination false} Enumerator<T> {
+    var signaledDone: bool
+    var hasFailed: bool
+    ghost const Repr: set<object>
+
+    predicate Valid() reads this, Repr ensures Valid() ==> this in Repr
+
+    method Next() returns (element: Result<Option<T>>)
+      requires Valid()
+      modifies Repr
+      ensures Valid()
+      ensures Repr == old(Repr)
+      ensures old(signaledDone) || old(hasFailed) ==> element.Failure?
+      ensures element.Failure? ==> hasFailed
+      ensures element.Success? && element.value.None? ==> signaledDone
+      // TODO If T is a seq, then whether it's interpreted as an element
+      // in some list of seq, or a chunk of a larger seq, depends on the
+      // implementation. There is a problem, however, where the latter
+      // is able to represent [] to mean "no data right now", while
+      // the former has no such mechanism. This feels like this interface
+      // half allows "no data right now", which seems bad.
+  }
+
+  trait {:termination false} Aggregator<T> {
+    ghost const Repr: set<object>
+    var signaledDone: bool
+    var hasFailed: bool
+
+    predicate Valid() reads this, Repr ensures Valid() ==> this in Repr
+
+    method Accept(element: T) returns (res: Result<bool>)
+      requires Valid()
+      modifies Repr
+      ensures Valid()
+      ensures Repr == old(Repr)
+      ensures old(signaledDone) || old(hasFailed) ==> res.Failure?
+      ensures res.Failure? ==> hasFailed
+      // TODO: Still not sure about allowing Success(false) here
+
+    method End() returns (res: Result<bool>)
+      requires Valid()
+      modifies Repr
+      ensures Valid()
+      ensures Repr == old(Repr)
+      ensures old(signaledDone) || old(hasFailed) ==> res.Failure?
+      ensures res.Failure? ==> hasFailed
+      ensures res.Success? && res.value ==> signaledDone
+      // TODO: Still not sure about allowing Success(false) here
+  }
+
+  // Native Enumerator implementation for enumerating bytes from a particular seq<T>
+  // in a specified chunk size
+  class SeqEnumerator<T> extends Enumerator<seq<T>> {
+    const s: seq<T>
+    ghost var enumerated: seq<T>
+    const chunkSize: nat
+    var i: nat
+
+    predicate Valid() reads this, Repr ensures Valid() ==> this in Repr
+    {
+      && i <= |s|
+      && chunkSize > 0
+      && enumerated == s[..i]
+      && this in Repr 
+    }
+
+    constructor (data: seq<T>, chunkSize: nat)
+      requires chunkSize > 0
+      ensures s == data
+      ensures enumerated == []
+      ensures !signaledDone
+      ensures !hasFailed
+      ensures i == 0
+      ensures this.chunkSize == chunkSize
+      ensures Valid() && fresh(Repr)
+    {
+        s := data;
+        enumerated := [];
+        signaledDone := false;
+        hasFailed := false;
+        i := 0;
+        this.chunkSize := chunkSize;
+        Repr := {this};
+    }
+    
+    method Next() returns (element: Result<Option<seq<T>>>)
+      requires Valid()
+      modifies Repr
+      ensures Valid()
+      ensures Repr == old(Repr)
+      ensures old(signaledDone) || old(hasFailed) ==> element.Failure?
+      ensures element.Failure? ==> hasFailed
+      ensures element.Success? && element.value.None? ==> signaledDone
+
+      /* Postconditions specific to SeqEnumerator */
+      ensures element.Success? && element.value.None? ==> i == |s|
+      ensures
+        var endSlice := Min(|s|, old(i)+chunkSize);
+        element.Success? && element.value.Some? ==> element.value.get == s[old(i)..endSlice]
+        && i == endSlice
+    {
+      if signaledDone {
+        hasFailed := true;
+        return Failure("Enumerator is at EOF and cannot be read.");
+      } else if hasFailed {
+        return Failure("Enumerator is in a failed state.");
+      } else if i >= |s| {
+        //EOF
+        signaledDone := true;
+        return Success(None());
+      }
+
+        
+      var endSlice := Min(|s|, i+chunkSize);
+      var data := s[i..endSlice];
+      i := endSlice;
+      enumerated := enumerated + data;
+      return Success(Some(data));
+    }
+  }
+
+  // Native Enumerator implementation for enumerating bytes from a particular seq<T>
+  // in a specified chunk size
+  class SeqAggregator<T> extends Aggregator<seq<T>> {
+    var s: seq<T>
+
+    predicate Valid() reads this, Repr ensures Valid() ==> this in Repr
+    {
+      this in Repr 
+    }
+
+    constructor ()
+      ensures !signaledDone
+      ensures !hasFailed
+      ensures Valid() && fresh(Repr)
+    {
+        s := [];
+        signaledDone := false;
+        hasFailed := false;
+        Repr := {this};
+    }
+
+    method Accept(element: seq<T>) returns (res: Result<bool>)
+      requires Valid()
+      modifies Repr
+      ensures Valid()
+      ensures Repr == old(Repr)
+      ensures old(signaledDone) || old(hasFailed) ==> res.Failure?
+      ensures res.Failure? ==> hasFailed
+    {
+      if signaledDone {
+        hasFailed := true;
+        return Failure("Aggregator has been ended and cannot accept any more data");
+      } else if hasFailed {
+        return Failure("Aggregator is in a failed state.");
+      }
+      s := s + element;
+      return Success(true);
+    }
+
+    method End() returns (res: Result<bool>)
+      requires Valid()
+      modifies Repr
+      ensures Valid()
+      ensures Repr == old(Repr)
+      ensures old(signaledDone) || old(hasFailed) ==> res.Failure?
+      ensures res.Failure? ==> hasFailed
+      ensures res.Success? && res.value ==> signaledDone
+    {
+      if signaledDone {
+        hasFailed := true;
+        return Failure("Aggregator is already at EOF");
+      } else if hasFailed {
+        return Failure("Aggregator is in a failed state.");
+      }
+      signaledDone := true;
+      return Success(true);
+    }
+  }
+}
