src/Util/ToyUTF8Transform.dfy
@@ -1,0 +1,393 @@
+include "../StandardLibrary/StandardLibrary.dfy"
+include "../StandardLibrary/UInt.dfy"
+include "../StandardLibrary/IO.dfy"
+include "UTF8.dfy"
+
+module {:extern "ToyUTF8Transform"} ToyUTF8Transform {
+  import opened StandardLibrary
+  import opened UInt = StandardLibrary.UInt
+  import IO
+  import Collections
+  import UTF8
+
+  // ToyEnumerator wraps and operates on an ExternBytesEnumerator
+  // Implements a toy example where we interpret read bytes as UTF8, duplicate
+  // each character (e.g. "abc" -> "aabbcc"), reencode the UTF8, and return those bytes.
+  class ToyEnumerator extends Collections.Enumerator<seq<uint8>> {
+    // Currently this specifies an ExternBytesEnumerator because we want to guarantee that
+    // we always get some bytes back on Next. This is needed in order to prove termination
+    // in the Dafny code (note that this just moves the termination concern into the extern).
+    // I see three possible paths forward here:
+    //    1. Don't prove termination in the Dafny code (this is honest, though we lose out an verifiying that
+    //       nothing specifically in the Dafny code results in some infinite loop)
+    //    2. Define a slightly more restrictive trait that extends Enumerator<seq<T>> with this property and use that 
+    var source: IO.ExternBytesEnumerator 
+    var utf8Transform: UTF8Transformer
+    var sourceAtEOF: bool
+
+    predicate Valid() reads this, Repr ensures Valid() ==> this in Repr
+    {
+      && this in Repr 
+      && source in Repr && source.Repr <= Repr && this !in source.Repr && source.Valid()
+      && utf8Transform in Repr && utf8Transform.Repr <= Repr && this !in utf8Transform.Repr && utf8Transform.Valid()
+      && utf8Transform.Repr !! source.Repr
+    }
+
+    constructor (source: IO.ExternBytesEnumerator)
+      requires source.Valid() 
+      ensures this.source == source
+      ensures !hasFailed
+      ensures !signaledDone
+      ensures Valid() && fresh(Repr - source.Repr - utf8Transform.Repr)
+    {
+      this.source := source;
+      this.sourceAtEOF := false;
+      this.hasFailed := false;
+      this.signaledDone := false;
+      var utf8Transform := new UTF8Transformer();
+      this.utf8Transform := utf8Transform;
+      this.Repr := {this} + source.Repr + utf8Transform.Repr;
+    }
+
+    method Next() returns (element: Result<Option<seq<uint8>>>)
+      requires Valid()
+      modifies Repr
+      ensures Valid()
+      ensures Repr == old(Repr)
+      ensures old(signaledDone) || old(hasFailed) ==> element.Failure?
+      ensures element.Failure? ==> hasFailed
+      ensures element.Success? && element.value.None? ==> signaledDone
+      // Ideally we could have condition here that describe the
+      // transformation we want, however this is based upon input
+      // that we don't get until runtime. Therefore, we verify
+      // that the Transform by itself is correct. Ideally we could
+      // leave less unspecified in this method
+    {
+      if signaledDone {
+        hasFailed := true;
+        return Failure("Enumerator is at EOF and cannot be read.");
+      } else if hasFailed {
+        return Failure("Enumerator is in a failed state.");
+      }
+
+      // Need to pull from the source and transform until we get back
+      // at least one byte to return, or Done
+      while true
+        decreases 4 - |utf8Transform.inBuffer|;
+        invariant Valid()
+      {
+        // Read from source
+        var res := source.Next();
+        if res.Failure? {
+          hasFailed := true;
+          return Failure("Failed ot read source");
+        } else if res.value.None? {
+          // Source is at EOF, we should trigger EOF through transformer
+          // and return the result
+          sourceAtEOF := true;
+          var transformed := utf8Transform.Final();
+          if transformed.Failure? {
+            hasFailed := true;
+            return Failure("Failed to end encryption operation");
+          }
+          signaledDone := true;
+          return Success(None());
+        }
+
+        // Transform bytes read from source
+        var transformed := utf8Transform.Transform(res.value.get);
+        if transformed.Failure? {
+          hasFailed := true;
+          return Failure("Failed to transform bytes");
+        } else if transformed.Success? && transformed.value.Some? {
+          return Success(Some(transformed.value.get));
+        }
+      }
+    }
+  }
+  
+  // ToyAggregator wraps and operates on an Aggregator
+  // Implements a toy example where we interpret input bytes as UTF8, duplicate
+  // each character (e.g. "abc" -> "aabbcc"), reencode the UTF8, and write those bytes.
+  class ToyAggregator extends Collections.Aggregator<seq<uint8>> {
+    // Again, we specify using ExternBytesAggregator instead of Aggregator
+    // because we want to be able to prove termination, and that requires
+    // restricting the interface from allowing "wait"s.
+    // Couple other solutions:
+    //    1. Check during runtime and fail if Success(false) is returned
+    //    2. Remove termination requirement from interface
+    //    3. Remove "wait" from interface
+    //    4. Define new "blocking" trait with this property which extends Aggregator
+    var sink: IO.ExternBytesAggregator
+    var utf8Transform: UTF8Transformer
+
+    predicate Valid() reads this, Repr ensures Valid() ==> this in Repr
+    {
+      && this in Repr 
+      && sink in Repr && sink.Repr <= Repr && this !in sink.Repr && sink.Valid()
+      && utf8Transform in Repr && utf8Transform.Repr <= Repr && this !in utf8Transform.Repr && utf8Transform.Valid()
+      && utf8Transform.Repr !! sink.Repr
+    }
+
+    constructor (sink: IO.ExternBytesAggregator)
+      requires sink.Valid() 
+      ensures this.sink == sink
+      ensures !hasFailed
+      ensures !signaledDone
+      ensures Valid() && fresh(Repr - sink.Repr - utf8Transform.Repr)
+    {
+      this.sink := sink;
+      this.hasFailed := false;
+      this.signaledDone := false;
+      var utf8Transform := new UTF8Transformer();
+      this.utf8Transform := utf8Transform;
+      this.Repr := {this} + sink.Repr + utf8Transform.Repr;
+    }
+
+    method Accept(element: seq<uint8>) returns (res: Result<bool>)
+      requires Valid()
+      modifies Repr
+      ensures Valid()
+      ensures Repr == old(Repr)
+      ensures old(signaledDone) || old(hasFailed) ==> res.Failure?
+      ensures res.Failure? ==> hasFailed
+      // Ideally we could have condition here that describe the
+      // transformation we want, however we have no way to look
+      // into what was written by the underlying Aggregator (it
+      // is impossible to do so and remain generic about the sink).
+      // Therefore, we verify that the Transform by itself is correct.
+      // Ideally we could leave less unspecified in this method
+    {
+      if signaledDone {
+        hasFailed := true;
+        return Failure("Enumerator is at EOF and cannot be read.");
+      } else if hasFailed {
+        return Failure("Enumerator is in a failed state.");
+      }
+
+      var transformedChunk := utf8Transform.Transform(element);
+      if transformedChunk.Failure? {
+        hasFailed := true;
+        return Failure("Failed to transform input");
+      } else if transformedChunk.value.None? {
+        // successfully accepted bytes into buffer, but not enough
+        // to write tranformation sink.
+        return Success(true);
+      }
+      
+      // Write the transformed bytes to the sink
+      res := sink.Accept(transformedChunk.value.get);
+      if res.Failure? {
+        hasFailed := true;
+        return Failure("Failed to write bytes to underlying sink.");
+      }
+      // There isn't a way to assert this as a postcondition on the method,
+      // but make sure that these bytes were actually written
+      // TODO: This seems like an easy miss.
+      assert res.Success? && res.value;
+
+      return res;
+    }
+
+    method End() returns (res: Result<bool>)
+      requires Valid()
+      modifies Repr
+      ensures Valid()
+      ensures Repr == old(Repr)
+      ensures old(signaledDone) || old(hasFailed) ==> res.Failure?
+      ensures res.Failure? ==> hasFailed
+      ensures res.Success? && res.value ==> signaledDone
+    {
+      if signaledDone {
+        hasFailed := true;
+        return Failure("The Aggregator has already completed.");
+      } else if hasFailed {
+        return Failure("The Aggregator is in a failed state.");
+      }
+
+      // End transformer. In our case, this will fail if extra bytes are in the buffer
+      var transformed := utf8Transform.Final();
+      if transformed.Failure? {
+        hasFailed := true;
+        return Failure("Failed to end transform due to extra invalid bytes");
+      } else if transformed.value.Some? {
+        // write final bytes to sink
+        var acceptRes := sink.Accept(transformed.value.get);
+        if acceptRes.Failure? {
+          hasFailed := true;
+          return Failure("Failled to write to sink");
+        } 
+        assert acceptRes.value;
+      }
+
+      // Signify End to Sink
+      res := sink.End();
+      if res.Failure? {
+        hasFailed := true;
+        return Failure("Failed to End underlying sink.");
+      }
+    
+      // TODO Same as above, this seems easy to not check
+      assert res.Success? && res.value;
+
+      signaledDone := true;
+      return res;
+    }
+  }
+
+  // Represents a stateful transformation of streamed input into transformed output.
+  // Maintains a buffer of inputted bytes, interprets those bytes as UTF8, and returns a sequence of bytes
+  // representing the encoding of those UTF8 characters doubled. E.g.: UTF8.Decode("abc") -> UTF8.Decode("aabbcc").
+  class UTF8Transformer {
+    ghost const Repr: set<object>
+    var done: bool
+    var hasFailed: bool
+    var inBuffer: seq<uint8>
+
+    predicate Valid() reads this, Repr ensures Valid() ==> this in Repr
+    {
+      && this in Repr 
+      && |inBuffer| < 4
+    }
+
+    constructor ()
+      ensures !hasFailed
+      ensures !done
+      ensures inBuffer == []
+      ensures Valid() && fresh(Repr)
+    {
+      this.hasFailed := false;
+      this.done := false;
+      this.inBuffer := [];
+      this.Repr := {this};
+    }
+
+    // Transforms inputted bytes into transformed output, and maintains a buffer of bytes for the input that
+    // is not yet transformed.
+    // If this method does not have enough bytes to interpret at least one UTF8 character, returns Success(None).
+    // If this method has enough bytes to determine that an invalid UTF8 encoding was inputted, returns Failure().
+    method Transform(element: seq<uint8>) returns (transformed: Result<Option<seq<uint8>>>)
+      requires Valid()
+      modifies Repr
+      ensures Valid()
+      ensures old(done) || old(hasFailed) ==> transformed.Failure?
+      ensures transformed.Failure? ==> hasFailed
+      // Note: It is very difficult to reason about the exact transform here due to the fact that UTF8.Encode/Decode goes to an
+      // extern method, meaning that we don't have any tools to reason about how we expect those transformations to go.
+      // Regardless, we can still specify things such that the below to at least ensure we do not fail on good inputs
+      ensures transformed.Success? && transformed.value.None? ==> |inBuffer| == |element| + |old(inBuffer)|
+      ensures transformed.Success? && transformed.value.Some? ==> UTF8.ValidUTF8Seq(transformed.value.get)
+      ensures
+        var newBuffer := old(inBuffer) + element;
+        && (!done && !hasFailed && |old(inBuffer)+element| > 0 && UTF8.ValidUTF8Seq(newBuffer) ==> transformed.Success? && transformed.value.Some?)
+        && (!done && !hasFailed && |old(inBuffer)+element| > 1 && UTF8.ValidUTF8Seq(newBuffer[..|newBuffer| - 1]) ==> transformed.Success? && transformed.value.Some?)
+        && (!done && !hasFailed && |old(inBuffer)+element| > 2 && UTF8.ValidUTF8Seq(newBuffer[..|newBuffer| - 2]) ==> transformed.Success? && transformed.value.Some?)
+        && (!done && !hasFailed && |old(inBuffer)+element| > 3 && UTF8.ValidUTF8Seq(newBuffer[..|newBuffer| - 3]) ==> transformed.Success? && transformed.value.Some?)
+    {
+      if done {
+        hasFailed := true;
+        return Failure("Transformer is at EOF and cannot transform any more.");
+      } else if hasFailed {
+        return Failure("Transformer is in a failed state.");
+      }
+
+      // This is a quick (to implement) and dirty way to determine what segment of the inBuffer is valid UTF8.
+      // We can assume that the first index is always the beginning of a UTF8 charactera, but we need
+      // to pick a slice such that the end index doesn't cut in the middle of a multi-byte UTF8 character.
+      // UTF8 characters can be up to four bytes, so just brute force by checking the last four indexes.
+      // If none of these work, then we know that the inputted bytes were not valid UTF8.
+      // If we don't have four bytes yet, and the indexes we do have aren't valid, return Success(None())
+      inBuffer := inBuffer + element;
+      assert inBuffer == old(inBuffer) + element;
+      var endIndex;
+      if (|inBuffer| > 0 && UTF8.ValidUTF8Seq(inBuffer)) {
+        endIndex := |inBuffer|;
+        assert inBuffer == inBuffer[..endIndex];
+        assert UTF8.ValidUTF8Seq(inBuffer[..endIndex]);
+      } else if (|inBuffer| > 1 && UTF8.ValidUTF8Seq(inBuffer[..|inBuffer| - 1])) {
+        endIndex := |inBuffer| - 1;
+        assert UTF8.ValidUTF8Seq(inBuffer[..endIndex]);
+      } else if (|inBuffer| > 2 && UTF8.ValidUTF8Seq(inBuffer[..|inBuffer| - 2])) {
+        endIndex := |inBuffer| - 2;
+        assert UTF8.ValidUTF8Seq(inBuffer[..endIndex]);
+      } else if (|inBuffer| > 3 && UTF8.ValidUTF8Seq(inBuffer[..|inBuffer| - 3])) {
+        endIndex := |inBuffer| - 3;
+        assert UTF8.ValidUTF8Seq(inBuffer[..endIndex]);
+      } else if |inBuffer| > 3 {
+        // if we get here, then the bytes we are reading are invalid UTF8
+        hasFailed := true;
+        inBuffer := [];
+        return Failure("Encountered invalid UTF8 bytes");
+      } else {
+        // otherwise, we don't have enough bytes to perform the transformatoin
+        // theyre already in the buffer, so return Success(None)
+        return Success(None());
+      }
+
+      // grab the chunk of bytes we want to work with and update the buffer
+      var chunkToManipulate := inBuffer[..endIndex];
+      inBuffer := inBuffer[endIndex..];
+
+      // Convert the chunk from UTF8 bytes -> string
+      var decodeRes := UTF8.Decode(chunkToManipulate);
+      if decodeRes.Failure? {
+        hasFailed := true;
+        return Failure("UTF8 Decoder encountered Failure: " + decodeRes.error);
+      }
+      var decodedChunk := decodeRes.value;
+
+      // iterate through decoded string to create new string which duplicates the characters
+      var chunkIndex := 0;
+      var doubledChunk := "";
+      while chunkIndex < |decodedChunk|
+      {
+        doubledChunk := doubledChunk + [decodedChunk[chunkIndex], decodedChunk[chunkIndex]];
+        chunkIndex := chunkIndex + 1;
+      }
+
+      // Convert back to bytes
+      var encodeRes := UTF8.Encode(doubledChunk);
+      if encodeRes.Failure? {
+        hasFailed := true;
+        return Failure("UTF8 Decoder encountered Failure: " + encodeRes.error);
+      }
+      var transformedChunk := encodeRes.value;
+      
+      // Return transformed bytes
+      return Success(Some(transformedChunk));
+    }
+
+    // Signifies the end of the transformer, processing any bytes remaining in the buffer
+    // and returning the final transformed bytes.
+    // If this method does not have enough bytes in the buffer to complete the transformation,
+    // returns Failure().
+    // Once called, UTF8Transformer will faill all future Final() or Transform() calls.
+    // Note: for this transform we never have final bytes to return, however I am modeling
+    // this such that bytes could be returned since we will need that behavior for the ESDK Encrypt/Decrypt
+    method Final() returns (res: Result<Option<seq<uint8>>>)
+      requires Valid()
+      modifies Repr
+      ensures Valid()
+      ensures res.Success? ==> done
+      ensures old(done) || old(hasFailed) ==> res.Failure?
+      ensures res.Failure? ==> hasFailed
+    {
+      if done {
+        hasFailed := true;
+        return Failure("The Aggregator has already completed.");
+      } else if hasFailed {
+        return Failure("The Aggregator is in a failed state.");
+      }
+
+      // If we still have things in the inBuffer, then the bytes inputted were not valid UTF8.
+      if |inBuffer| > 0 {
+        hasFailed := true;
+        return Failure("Invalid UTF8 bytes supplied to transformer.");
+      }
+
+      // Otherwise, we don't have any bytes to return, so return Success(None)
+      done := true;
+      return Success(None());
+    }
+  }
+}
